Examples/counter.v
@@ -1,0 +1,143 @@
+From mathcomp Require Import ssreflect ssrbool ssrfun ssrnat eqtype seq.
+From fcsl Require Import axioms pred.
+From fcsl Require Import pcm unionmap heap.
+From HTT Require Import domain stmod stsep stlog stlogR.
+Set Implicit Arguments.
+Unset Strict Implicit.
+Unset Printing Implicit Defensive.
+Obligation Tactic := auto.
+
+(* counter that hides local state with an abstract predicate *)
+
+Prenex Implicits exist.
+
+Record cnt : Type :=
+  Counter {inv : nat -> Pred heap;
+           method : {v : nat}, STsep (inv v,
+                                [vfun (y : nat) h => y = v /\ inv (v.+1) h])}.
+
+(*
+Lemma gw A x (v : A) : valid (x :-> v) -> (x :-> v) \In (pts x v).
+Proof. by move=>A x v H; rewrite opn. Qed.
+
+Hint Resolve gw.
+*)
+Program Definition new : STsep (emp, [vfun v => inv v 0]) :=
+  Do (x <-- alloc 0;
+      ret (@Counter (fun v h => h = x :-> v)
+                    (Do (y <-- !x;
+                        x ::= y.+1;;
+                        ret y)))).
+Next Obligation.
+move=>x ? /= [y]->.
+do 3!step; move=>V1 z H; rewrite validPt in V1.
+suff: (y = z) by move=>->.
+apply: (@hcancelPtV _ x)=>//.
+by rewrite validPt.
+Qed.
+Next Obligation.
+move=>? /= ->. apply: bnd_seq. apply: val_alloc.
+
+apply (@bnd_allocR _ cnt (fun x => ret {|
+                                           inv := fun v : nat => eq^~ (x :-> v);
+                                           method := Do y <-- ! x; x ::= y.+1;; ret y
+                                         |}) 0 Unit).
+case: H=><-; apply: bnd_alloc=>// x; heval=>D; hhauto; rewrite unh0 /= in D *; auto.
+Qed.
+
+(* Hiding local state with an abstract predicate is logically expensive,  *)
+(* as the resulting abstract package must have a large type (since it     *)
+(* includes a heap predicate). Hence, the package cannot be stored into   *)
+(* the heap.                                                              *)
+(*                                                                        *)
+(* This is not particularly hurtful in the current model, since the model *)
+(* assigns large types to computations anyway. But the later can easily   *)
+(* be changed using the Petersen-Birkedal denotational model.             *)
+(*                                                                        *)
+(* Once we switch to the new model, we can hide the local state of the    *)
+(* object by abstracting over the "representation" of the inv predicate,  *)
+(* as follows.                                                            *)
+
+Inductive rep : Type := Rep of loc & nat.
+Definition ptr r := let: Rep l _ := r in l.
+Definition val r := let: Rep _ v := r in v.
+Definition interp (r : rep) : Rel heap := [Rel h | h \In ptr r --> val r].
+
+Record scnt : Type :=
+  SCount {sinv : nat -> rep;
+          smethod : STsep nat (fun i => exists v, i \In interp (sinv v),
+                               fun y i m => forall v, i \In interp (sinv v) ->
+                                 y = Val v /\ m \In interp (sinv v.+1))}.
+
+Program
+Definition snew : STsep scnt (emp, fun y i m =>
+                                     exists v, y = Val v /\ m \In interp (sinv v 0)) :=
+  Do (x <-- alloc 0;
+      ret (@SCount (fun v => Rep x v)
+                    (Do (y <-- !x;
+                        x ::= y.+1;;
+                        ret y)))).
+Next Obligation.
+by case/swp: H0=>->; heval=>D1 w; case/opn=>D; heap_cancel=>//= _ _ ->; rewrite InE /= opn.
+Qed.
+Next Obligation.
+by case: H=><-; apply: bnd_alloc=>// x; heval=>D; hhauto; rewrite unh0 InE /= opn in D *.
+Qed.
+
+(* This solution replaces the abstract predicate inv with a type of     *)
+(* representations, and a semantic function that interprets the         *)
+(* representation into a predicate. We will typically want to prevent   *)
+(* clients from looking at the representation, which can be done either *)
+(* by making the type rep abstract, or by using some kind of            *)
+(* computational irrelevance to make the sinv component of scnd         *)
+(* inaccessible to programs. One possible solution for the later is to  *)
+(* add new irrelevance constructors into type theory, as                *)
+(* suggested by Pfenning, or Barras.                                    *)
+(*                                                                      *)
+(* Or, one can choose inv to have the type nat -> rep -> Prop, as shown *)
+(* below. The type nat -> rep -> Prop is still a small type (it doesn't *)
+(* quantify over heaps). So a package containing such an invariant will *)
+(* be storable in the heap.                                             *)
+
+Definition pinterp (R : rep -> Prop) : Rel heap :=
+  [Rel h | forall r, R r -> h \In ptr r --> val r].
+
+Record pcnt : Type :=
+  PCount {pinv : nat -> rep -> Prop;
+          pmethod : STsep nat (fun i => exists v, i \In pinterp (pinv v),
+                               fun y i m => forall v, i \In pinterp (pinv v) ->
+                                 y = Val v /\ m \In pinterp (pinv v.+1))}.
+
+Program
+Definition pnew : STsep pcnt (emp, fun y i m =>
+                                     exists v, y = Val v /\ m \In pinterp (pinv v 0)) :=
+  Do (x <-- alloc 0;
+      ret (@PCount (fun v r => r = Rep x v)
+                    (Do (y <-- !x;
+                        x ::= y.+1;;
+                        ret y)))).
+Next Obligation.
+case/swp: {H0} (H0 (Rep x H) (refl_equal _))=>->; heval=>D w.
+move/(_ (Rep x w) (refl_equal _)); case/opn=>D1; heap_cancel=>//= _ _ ->.
+by split=>//= r ->; auto.
+Qed.
+Next Obligation.
+case: H=><-; apply: bnd_alloc=>// x; heval=>D; hhauto; rewrite InE unh0 in D *.
+move=>r -> /=; auto.
+Qed.
+
+(* Of course, the solution is still not quite abstract, since one cannot   *)
+(* store the interpretation function together with the package, but that   *)
+(* seems unavoidable due to the restrictions of impredicativity.  We have  *)
+(* still gained something by using representations, however; we have made  *)
+(* programs with local state storable -- something that is not possible    *)
+(* if we use abstraction over heap predicates.                             *)
+(*                                                                         *)
+(* An altogether different approach is to define heaps as storing not      *)
+(* types, but type representations, with a global interpretation           *)
+(* function. The later, being global, will not need to be stored into      *)
+(* heaps. Then heaps will be a small type, and we can freely abstract over *)
+(* them. This lifts the representation approach to a global level, making  *)
+(* it potentially more uniform, but it also makes it seemingly much more   *)
+(* difficult.                                                              *)
+
